```
(1) = b !- a = (b - a) * (1 + q_1)
(2) = t !* (b !- a) = t * (b - a) * (1 + q_1) * (1 + q_2)
(3) = a !+ t !* (b !- a) = a * (1 + q_3) + t * (b - a) * (1 + q_1) * (1 + q2) * (1 + q3)  

(4) = (1.f !- t) = (1 - t) * (1 + q_4)  
(5) = (1.f !- t) !* a = (1 - t) * a * (1 + q_4) * (1 + q_5)  
(6) = t !* b = t * b * (1 + q6)  
(7) = (1.f !- t) !* a !+ t !* b = ((1 - t) * a * (1 + q_4) * (1 + q_5) + t * b * (1 + q6)) * (1 + q_7)  

При b = a,  
(3) = a !+ (2) = a, т.к при сложении с нулем не будет погрешности   
(7) = a * (1 + q7) * ((1 - t) * (1 + q_4) * (1 + q_5) + t * (1 + q6))   

При t = 1.f,  
(1) = a !+ (2) = a !+ (b !- a) = (a + (b - a) * (1 + q_1)) * (1 + q_3) = (b + (b - a) * q_1) * (1 + q_3)
(2) = (5) !+ (6) = 0 + b = b, т.к. при умножении на 1 и при сложении с 0 не будет погрешности
```